Applying Function Transformations
-------

Recall the various function transformations:

* vertical shift
* horizontal shift
* vertical stretche or compressions
* horizontal stretches or compressions
* reflection along the x-axis and/or y-axis

When any combinations of these transformations are applied to $f(x)$ to obtain $g(x)$, we get $g(x) = af(k(x - h)) + c$.


Here is what it looks like for $f(x) = x$, $f(x) = x^2$, $f(x) = \frac{1}{x}$, $f(x) = \sqrt{x}$, and $f(x) = \abs{x}$.

| Parent Function | Transformed Function |
| --- | --- |
| $f(x) = x$ | $g(x) = a(k(x - h)) + c$ |
| $f(x) = x^2$ | $g(x) = a(k(x - h))^2 + c$ |
| $f(x) = \frac{1}{x}$ | $g(x) = \frac{a}{(k(x - h))} + c$ |
| $f(x) = \sqrt{x}$ | $g(x) = a\sqrt{k(x - h)} + c$ |
| $f(x) = \abs{x}$ | $g(x) = a\abs{k(x - h)} + c$ |

The image of a point $(x, y)$ in a function is the point $(\frac{x}{k} + h, ay + c)$ on the transformed function.


Describe the transformation of each of the following functions from g(x).

1. $\frac{g(2x)}{3} - 3$

2. $3g(x - 2) + 4$

3. $\frac{g(-2x)}{3}$


Describe the transformation of each of the following functions from its parent function, and find the image of the origin.

1. $f(x) = \frac{-x}{2} + 4$

2. $f(x) = 3(2x)^2 - 3$

3. $f(x) = \sqrt{-3(x + 3)}$

4. $f(x) = \abs{-2x - 8)}$

