Adding and Subtracting Polynomials
-------
 
### Adding Polynomials

Recall that we can simplify polynomials by adding the like terms. 

Example: Simplify $4 + x - 3x$.

$x$ and $-3x$ are like terms. Since $x + (-3x) = 2x$, the polynomial simplifies to $4 - 2x$.

To add two polynomials, we first combine them into one polynomial, then we simplify it. 

Example: Add $3 + 4x$ and $-7 + 2x + x^2$.

$(3 + 4x) + (-7 + 2x + x^2) = 3 + 4x + -7 + 2x + x^2 = -4 + 6x + x^2$.

Example: What is the sum of $1 + 3x + 2x^2$ and $2 - 2x + x^2$?

$(1 + 3x + 2x^2) + (2 - 2x + x^2) = 1 + 3x + 2x^2 + 2 - 2x + x^2 = 1 + 2 + 3x - 2x + 2x^2 + x^2 = 3 + x + 3x^2$.

Add the following polynomials.

1. $1 + 2x + 3x^2$ and $4 + 2x + x^2$

2. $2 + x^3$ and $4 + x^2 + 2x^3$

3. $x^3 + x^2$ and $3x^3 + 1$.


### Subtracting Polynomials

In order to subtract polynomials, we first have to understand that we cannot simply combine them with a subtraction sign instead of an addition sign like we do when adding polynomials. When a polynomial is subtracted from another, every single one of its terms is subtracted, so we have to negate each term before combining the two polynomials.

Example: Subtract $3 + 4x$ and $-7 + 2x + x^2$.

$(3 + 4x) - (-7 + 2x + x^2) = (3 + 4x) + (7 - 2x - x^2) = 3 + 4x + 7 - 2x - x^2 = 10 + 2x - x^2$.

Example: Find the the difference between $1 + 3x + 2x^2$ and $2 - 2x + x^2$.

$(1 + 3x + 2x^2) - (2 - 2x + x^2) = (1 + 3x + 2x^2) + (-2 + 2x - x^2) = 1 + 3x + 2x^2 - 2 + 2x - x^2 = 1 - 2 + 3x + 2x + 2x^2 - x^2 = -1 + 5x + x^2$.

Subtract the following polynomials.

1. $1 + 2x + 3x^2$ and $4 + 2x + x^2$

2. $2 + x^3$ and $4 + x^2 + 2x^3$

3. $x^3 + x^2$ and $3x^3 + 1$.