Factoring Trinomials and Binomials
-------

### Definitions

* A **factor of a term** is another term that divides into the term. Example: $2x$ is a factor of $4x$ since $2x \times 2 = 4x$.

* A **factor of a polynomial** is a term or polynomial that divides into the polynomial. Example: $2x + 1$ is a factor of $2x^2 + 5x + 2$ since $(2x + 1)(x + 2)= 2x^2 + 5x + 2$.
 
* A **root of a polynomial** is a value of its variables that results in the polynomial evaluating to zero. A root can also be called a **zero**. Example: $x = \frac{-1}{2}$ is a root of $2x^2 + 5x + 2$ since $2(\frac{-1}{2})^2 + 5(\frac{-1}{2}) + 2 = 0$.

* **Factoring a polynomial** is the process of changing it from a sum of terms to a product of factors. Example: $(2x + 1)(x + 2)$ is the factored form of $x^2 + 5 + 2$.


List all the factors of each of the following terms. 

1. $2x^2$

2. $5xy$

 
### Common Factors

One way of factoring a polynomial is to find the **greatest common factor** among all the terms. For example, we can factor $3xy + 6x^2 + 12xy^2$ using the common factor 3x to get $3xy + 6x^2 + 12xy^2 = 3x(y + 2x + 4y^2)$. 3 and $x$ are also common factors of each of the terms in the polynomial, but $3x$ is the greatest common factor.

Factor each of the following polynomials using the greatest common factor among all the terms.

1. $4x + 2x^2 + 6x^3$

2. $6 + 3x + 6x^2$


### Factoring $x^2 + bx + c$

To factor a trinomial in the form $x^2 + bx + c$, we need to find its roots. If it does have roots, say $s$ and $t$, they will have the following property: $s + t = b$ and $st = c$. When we find $s$ and $t$, the factored form is simply $(x - s)(x - t)$.

For example, we can factor $x^2 + 5x - 14$ by determining through guess-and-check that $7 + (-2) = 5$ and $7 \times -2 = -14$, so $x^2 + 5x - 14 = (x + 7)(x - 2)$.

Not all trinomials in the form $x^2 + bx + c$ has roots. The ones that do not have any cannot be factored.

Factor each of the following polynomials.

1. $x^2 + 7x + 10$

2. $x^2 - 3x - 18$


### Factoring $ax^2 + bx + c$

To factor a trinomial in the form $ax^2 + bx + c$, we can follow a similar process as when $a = 1$, but with some extra steps.

1. Find two constants, $s$ and $t$, that have the property $s + t = b$, $st = ac$. If $s$ and $t$ do not exist, it cannot be factored.
2. Rewrite $ax^2 + bx + c$ as $ax^2 + sx + tx + c$.
3. Rewrite it by factoring $ax^2 + sx$, then factoring $tx + c$. There will be a common factor among both of them.
4. Factor out the common factor.

Here is an example using $2x^2 + 5x + 2$.

We want two constants $s$ and $t$ such that $s + t = 5$ and $st = 4$. The solution $s = 1$ and $t = 4$ works. We could also use $s = 4$ and $t = 1$.
$2x^2 + 5x + 2 = 2x^2 + x + 4x + 2 = x(2x + 1) + 2(2x + 1)= (2x + 1)(x + 2)$.


Factor each of the following polynomials.

1. $2x^2 - 3x - 9$

2. $2x^2 - 11x + 5$


### Difference of Squares

A **square** is a term that can be written as another term squared. Example: $4x^2$ is a square since $(2x)^2 = 4x^2$.

When a binomial is a difference of squares, it can always be factored. $a^2 - b^2 = (a - b)(a + b)$, where $a$ and $b$ are both terms.

For example, $9x^2 - 4 = (3x - 2)(3x + 2)$, and $16x^4 - x^2 = (4x^2 - x)(4x^2 + x)$.

Factor each of the following polynomials.

1. $4x^2 - 9$

2. $9x^2y^2 - 16$