Trigonometric Identities
-------

An **identity** is an equation that holds true for every value in the variables' domains. **Trigonometric identities** are identities that involve trigonometric ratios.

### Pythagorean Identity

Since the unit circle has the equation $x^2 + y^2 = 1$, substituting $(sin\theta, cos\theta)$ gives us a useful identity: $sin^2\theta+ cos^2\theta = 1$ for all values of $\theta$. This is called a **Pythagorean Identity** since the equation $x^2 + y^2 = 1$ creating the unit circle is a result of the Pythagorean Theorem.

$sin^2\theta$ is the conventional way to write $(sin\theta)^2$, and same goes for $cos^2\theta$. 


### Reciprocal Identitites

Recall the reciprocal trigonometric ratios: cosecant ($csc$), secant ($sec$), and cotangent ($cot$).

The reciprocal identities are the following: $sin\theta = \frac{1}{csc\theta}, cos\theta = \frac{1}{sec\theta}, and tan\theta = \frac{1}{cot\theta\theta)$.

It may help to remember that the reciprocal of a ratio starting with "co" does not start with "co".


### Quotient Identity

If we substitute $sin\theta = \frac{OPP}{HYP}$ and $cos\theta = \frac{ADJ}{HYP}$ from SOHCAHTOA into $\frac{sin\theta}{cos\theta}$, we get $\frac{sin\theta}{cos\theta} = \frac{\frac{OPP}{HYP}{\frac{ADJ}{HYP} = \frac{OPP}{HYP} \times \frac{HYP}{ADJ} = \frac{OPP}{ADJ} = tan\theta$. This gives us the quotient identity $\frac{sin\theta}{cos\theta} = tan\theta$.


### Proving Identities

We can prove a new trigonometric identnties by substituting in known identities. For example, we can prove that $sin\theta sec\theta = tan\theta$ by substititing in a reciprocal identity on the left side, then using the quotient identity to simplify.

$sin\theta sec\theta = sin\theta \frac{1}{cos\theta} = \frac{sin\theta}{cos\theta} = tan\theta$.

It is important to not assume that both sides are equivelant. We choose one side, and rewrite it until it becomes the other side.


Prove each of the following trigonometric identnties.

1. $sin^2⁡\theta+cos^2\theta = sec^2⁡\theta − tan^2\theta$.

2. $\frac{sin^2\theta}{tan^2\theta} + sin^2\theta = sin^2\theta csc^2 \theta$.
