Negative Exponents and Reciprocals
-------

### Negative Exponents

Recall the Product of Powers rule: $a^n \times a^m = a^{m + n}$.

Let $\frac{1}{a}^m = a^n$. Since $(\frac{1}{a}^m) \times a^m = 1$, we can write $a^n \times a^m = a^{n+m} = a^0 = 1$. By the product rule, $n + m = 0$, giving $-n = m$.

This gives us the rule $\frac{1}{a^n} = = a^{-n}$. When $n = 1$, this gives us the Negative Power rule:t $\frac{1}{a} = = a^{-1}$

We can use this to prove the Negative Power of Quotient rule: $(\frac{a}{b})^{-1} = \frac{b}{a}$.

$(\frac{a}{b}^n)^{-1} = \frac{1}{\frac{a}{b}} = 1 \div \frac{a}{b} = 1 \times \frac{b}{a} = \frac{1}{\frac{b}{a}}$.


Rewrite each of the expressions as a fraction using only positive exponents, then evaluate by substituting $x = 3$.

1. $2^{-x}$

2. $3^{x + 1} \times 2^{-x}$

3. $\frac{3^x}{5 \times 2^{-(x-1)}}$

4. $4^x \times $\frac{3^{-(x+1)}}{5 \times 4^{x + 2}$$