Power Rules
-------

### Product Rules

Product of Powers: a^n × a^m = a^(n + m)

Proof:
a^n × a^m = (a × a × ... × a)_{n times} (a × a × ... × a)_{m times} =  (a × a × ... × a)_{m + n times} = a^(n + m)

Powers of Products: a^n × b^n = (ab)^n

Proof:
a^n × b^n = (a × a × ... × a)_{n times} (b × b × ... × b)_{n times} =  (ab × ab × ... × ab)_{n times} = (ab)^n


### Quotient Rules

Quotient of Powers: a^n / a^m = a^(n - m)

Proof:
a^n / a^m = (a × a × ... × a)_{n times} / (a × a × ... × a)_{m times} =  (a × a × ... × a)_{m - n times} = a^(m - n)

Power of Quotients: (a/b)^n = a^n/b^n

Proof:
(a/b)^n  = (a/b × a/b × ... × a/b)_{n times} = (a × a × ... × a)_{n times} / (b × b × ... × b)_{n times} = a^n / b^n


### Power Rule

Power of Powers: (a^n)^m = a^(nm)

Proof:
(a^n)^m = (a^n × a^n × ... × a^n)_{m times} = ((a × a × ... × a)_{n times})_{m times} = (a × a × ... × a)_{nm times} = a^(nm)


Although we just proved that these rules work for natural numbers, they all work for all real values of n and m, with a few restrictions on a and b. In some cases, a and b can't be both negative. We also cannot have values where we divide by 0 or evaluate 0^0.

We will be deriving other exponent rules using these ones.