Factoring Trinomials and Binomials
-------

### Definitions
* A **factor of a term** is another term that divides into the term.

 Example: 2x is a factor of 4x since 2x × 2 = 4x.

* A **factor of a polynomial** is a term or polynomial that divides into the polynomial.

 Example: 2x + 1 is a factor of 2x^2 + 5x + 2 since (2x + 1)(x + 2)= 2x^2 + 5x + 2.
 
* A **root of a polynomial** is a value of its variables that results in the polynomial evaluating to zero. A root can also be called a **zero**.

 Example: x = -1/2 is a root of 2x^2 + 5x + 2 since 2(-1/2)^2 + 5(-1/2) + 2 = 0.

 * **Factoring a polynomial** is the process of changing it from a sum of terms to a product of factors.
 
 Example: (2x + 1)(x + 2) is the factored form of x^2 + 5 + 2.

 
### Common Factors
One way of factoring a polynomial is to find a common factor among all the terms. For example, we can factor 3xy + 6x^2 + 12xy^2 using the common factor 3x to get 3xy + 6x^2 + 12xy^2 = 3x(y + 2x + 4y^2).


### Factoring x^2 + bx + c
To factor a trinomial in the form x^2 + bx + c, we need to find its roots. If it does have roots, say s and t, they will have the following property: s + t = b and st = c. When we find s and t, the factored form is simply (x - s)(x - t).

For example, we can factor x^2 + 5x - 14 by determining through guess-and-check that 7 + (-2) = 5 and 7 × -2 = -14, so x^2 + 5x - 14 = (x + 7)(x - 2).

Not all trinomials in the form x^2 + bx + c has roots. The ones that do not have any cannot be factored.


### Factoring ax^2 + bx + c
To factor a trinomial in the form ax^2 + bx + c, we can follow a similar process as when a = 1, but with some extra steps.

1. Find two constants, s and t, that have the property s + t = b, st = ac. If s and t do not exist, it cannot be factored.
2. Rewrite ax^2 + bx + c as ax^2 + sx + tx + c.
3. Rewrite it by factoring ax^2 + sx, then factoring tx + c. There will be a common factor among both of them.
4. Factor out the common factor.

Here is an example using 2x^2 + 5x + 2.

We want two constants s and t such that s + t = 5 and st = 4. The solution s = 1 and t = 4 works. We could also use s = 4 and t = 1.
2x^2 + 5x + 2 = 2x^2 + x + 4x + 2 = x(2x + 1) + 2(2x +1)= (2x + 1)(x + 2).


### Difference of Squares

* A **square** is a term that can be written as another term squared.

 Example: 4x^2 is a square since (2x)^2 = 4x^2.

When a binomial is a difference of squares, it can always be factored. a^2 - b^2 = (a-b)(a+b), where a and b are both terms.

For example, 9x^2 - 4 = (3x - 2)(3x + 2), and 16x^4 - x^2 = (4x^2 - x)(4x^2 + x)